<?xml version="1.0" encoding="UTF-8"?>
<!DOCTYPE rdf:RDF [
	<!ENTITY dct "http://purl.org/dc/terms/">
	<!ENTITY fibo-be-le-lp "https://spec.edmcouncil.org/fibo/ontology/BE/LegalEntities/LegalPersons/">
	<!ENTITY fibo-cae-ce-act "https://spec.edmcouncil.org/fibo/ontology/CAE/CorporateEvents/CorporateActions/">
	<!ENTITY fibo-fbc-fi-fi "https://spec.edmcouncil.org/fibo/ontology/FBC/FinancialInstruments/FinancialInstruments/">
	<!ENTITY fibo-fnd-arr-cls "https://spec.edmcouncil.org/fibo/ontology/FND/Arrangements/ClassificationSchemes/">
	<!ENTITY fibo-fnd-arr-lif "https://spec.edmcouncil.org/fibo/ontology/FND/Arrangements/Lifecycles/">
	<!ENTITY fibo-fnd-dt-oc "https://spec.edmcouncil.org/fibo/ontology/FND/DatesAndTimes/Occurrences/">
	<!ENTITY fibo-fnd-rel-rel "https://spec.edmcouncil.org/fibo/ontology/FND/Relations/Relations/">
	<!ENTITY fibo-fnd-utl-av "https://spec.edmcouncil.org/fibo/ontology/FND/Utilities/AnnotationVocabulary/">
	<!ENTITY lcc-cr "https://www.omg.org/spec/LCC/Countries/CountryRepresentation/">
	<!ENTITY lcc-lr "https://www.omg.org/spec/LCC/Languages/LanguageRepresentation/">
	<!ENTITY owl "http://www.w3.org/2002/07/owl#">
	<!ENTITY rdf "http://www.w3.org/1999/02/22-rdf-syntax-ns#">
	<!ENTITY rdfs "http://www.w3.org/2000/01/rdf-schema#">
	<!ENTITY skos "http://www.w3.org/2004/02/skos/core#">
	<!ENTITY sm "http://www.omg.org/techprocess/ab/SpecificationMetadata/">
	<!ENTITY xsd "http://www.w3.org/2001/XMLSchema#">
]>
<rdf:RDF xml:base="https://spec.edmcouncil.org/fibo/ontology/CAE/CorporateEvents/CorporateActions/"
	xmlns:dct="http://purl.org/dc/terms/"
	xmlns:fibo-be-le-lp="https://spec.edmcouncil.org/fibo/ontology/BE/LegalEntities/LegalPersons/"
	xmlns:fibo-cae-ce-act="https://spec.edmcouncil.org/fibo/ontology/CAE/CorporateEvents/CorporateActions/"
	xmlns:fibo-fbc-fi-fi="https://spec.edmcouncil.org/fibo/ontology/FBC/FinancialInstruments/FinancialInstruments/"
	xmlns:fibo-fnd-arr-cls="https://spec.edmcouncil.org/fibo/ontology/FND/Arrangements/ClassificationSchemes/"
	xmlns:fibo-fnd-arr-lif="https://spec.edmcouncil.org/fibo/ontology/FND/Arrangements/Lifecycles/"
	xmlns:fibo-fnd-dt-oc="https://spec.edmcouncil.org/fibo/ontology/FND/DatesAndTimes/Occurrences/"
	xmlns:fibo-fnd-rel-rel="https://spec.edmcouncil.org/fibo/ontology/FND/Relations/Relations/"
	xmlns:fibo-fnd-utl-av="https://spec.edmcouncil.org/fibo/ontology/FND/Utilities/AnnotationVocabulary/"
	xmlns:lcc-cr="https://www.omg.org/spec/LCC/Countries/CountryRepresentation/"
	xmlns:lcc-lr="https://www.omg.org/spec/LCC/Languages/LanguageRepresentation/"
	xmlns:owl="http://www.w3.org/2002/07/owl#"
	xmlns:rdf="http://www.w3.org/1999/02/22-rdf-syntax-ns#"
	xmlns:rdfs="http://www.w3.org/2000/01/rdf-schema#"
	xmlns:skos="http://www.w3.org/2004/02/skos/core#"
	xmlns:sm="http://www.omg.org/techprocess/ab/SpecificationMetadata/"
	xmlns:xsd="http://www.w3.org/2001/XMLSchema#">
	
	<owl:Ontology rdf:about="https://spec.edmcouncil.org/fibo/ontology/CAE/CorporateEvents/CorporateActions/">
		<rdfs:label xml:lang="en">Corporate Actions Ontology</rdfs:label>
		<dct:abstract>This ontology provides a high level overview of actions including corporate, market, and regulatory actions, ranging from business oriented events such as address and name changes, to those that are more specific to securities.</dct:abstract>
		<dct:license rdf:datatype="&xsd;anyURI">http://opensource.org/licenses/MIT</dct:license>
		<sm:contentLanguage rdf:resource="https://www.w3.org/TR/owl2-quick-reference/"/>
		<sm:copyright>Copyright (c) 2016-2022 EDM Council, Inc.</sm:copyright>
		<sm:dependsOn rdf:datatype="&xsd;anyURI">https://spec.edmcouncil.org/fibo/ontology/BE/</sm:dependsOn>
		<sm:dependsOn rdf:datatype="&xsd;anyURI">https://spec.edmcouncil.org/fibo/ontology/FBC/</sm:dependsOn>
		<sm:dependsOn rdf:datatype="&xsd;anyURI">https://spec.edmcouncil.org/fibo/ontology/FND/</sm:dependsOn>
		<sm:dependsOn rdf:datatype="&xsd;anyURI">https://www.omg.org/spec/LCC/</sm:dependsOn>
		<sm:fileAbbreviation>fibo-cae-ce-act</sm:fileAbbreviation>
		<sm:filename>CorporateActions.rdf</sm:filename>
		<owl:imports rdf:resource="https://spec.edmcouncil.org/fibo/ontology/BE/LegalEntities/LegalPersons/"/>
		<owl:imports rdf:resource="https://spec.edmcouncil.org/fibo/ontology/FBC/FinancialInstruments/FinancialInstruments/"/>
		<owl:imports rdf:resource="https://spec.edmcouncil.org/fibo/ontology/FND/Arrangements/ClassificationSchemes/"/>
		<owl:imports rdf:resource="https://spec.edmcouncil.org/fibo/ontology/FND/Arrangements/Lifecycles/"/>
		<owl:imports rdf:resource="https://spec.edmcouncil.org/fibo/ontology/FND/DatesAndTimes/Occurrences/"/>
		<owl:imports rdf:resource="https://spec.edmcouncil.org/fibo/ontology/FND/Relations/Relations/"/>
		<owl:imports rdf:resource="https://spec.edmcouncil.org/fibo/ontology/FND/Utilities/AnnotationVocabulary/"/>
		<owl:imports rdf:resource="https://www.omg.org/spec/LCC/Countries/CountryRepresentation/"/>
		<owl:imports rdf:resource="https://www.omg.org/spec/LCC/Languages/LanguageRepresentation/"/>
		<owl:versionIRI rdf:resource="https://spec.edmcouncil.org/fibo/ontology/CAE/20220301/CorporateEvents/CorporateActions/"/>
		<fibo-fnd-utl-av:hasMaturityLevel rdf:resource="&fibo-fnd-utl-av;Release"/>
	</owl:Ontology>
	
	<owl:Class rdf:about="&fibo-cae-ce-act;Action">
		<rdfs:subClassOf rdf:resource="&fibo-fnd-dt-oc;Occurrence"/>
		<rdfs:subClassOf>
			<owl:Restriction>
				<owl:onProperty rdf:resource="&fibo-fnd-rel-rel;appliesTo"/>
				<owl:someValuesFrom>
					<owl:Class>
						<owl:unionOf rdf:parseType="Collection">
							<rdf:Description rdf:about="&fibo-be-le-lp;LegalEntity">
							</rdf:Description>
							<rdf:Description rdf:about="&fibo-fbc-fi-fi;Security">
							</rdf:Description>
						</owl:unionOf>
					</owl:Class>
				</owl:someValuesFrom>
			</owl:Restriction>
		</rdfs:subClassOf>
		<rdfs:subClassOf>
			<owl:Restriction>
				<owl:onProperty rdf:resource="&lcc-cr;isClassifiedBy"/>
				<owl:someValuesFrom rdf:resource="&fibo-cae-ce-act;ActionClassifier"/>
			</owl:Restriction>
		</rdfs:subClassOf>
		<rdfs:label xml:lang="en">action</rdfs:label>
		<skos:definition xml:lang="en">event announced, initiated or carried out by an organization that affects a legal entity or the securities it issues and may have a material impact on that entity&apos;s stakeholders, such as shareholders and creditors</skos:definition>
		<skos:example xml:lang="en">Actions that impact an entity may be initiated by an issuer, exchange, regulator, creditor, or other third party.</skos:example>
		<fibo-fnd-utl-av:explanatoryNote xml:lang="en">Actions initiated by an issuer are typically approved by that company&apos;s board of directors and authorized by their shareholders.</fibo-fnd-utl-av:explanatoryNote>
	</owl:Class>
	
	<owl:Class rdf:about="&fibo-cae-ce-act;ActionClassificationScheme">
		<rdfs:subClassOf rdf:resource="&fibo-fnd-arr-cls;ClassificationScheme"/>
		<rdfs:subClassOf rdf:resource="&lcc-lr;CodeSet"/>
		<rdfs:subClassOf>
			<owl:Restriction>
				<owl:onProperty rdf:resource="&lcc-lr;hasMember"/>
				<owl:allValuesFrom rdf:resource="&fibo-cae-ce-act;ActionClassifier"/>
			</owl:Restriction>
		</rdfs:subClassOf>
		<rdfs:subClassOf>
			<owl:Restriction>
				<owl:onProperty rdf:resource="&fibo-fnd-rel-rel;defines"/>
				<owl:someValuesFrom rdf:resource="&fibo-cae-ce-act;ActionClassifier"/>
			</owl:Restriction>
		</rdfs:subClassOf>
		<rdfs:label>action classification scheme</rdfs:label>
		<skos:definition>scheme for classifying the kinds of actions and events that may be announced, initiated or carried out by an organization that affects a legal entity or the securities it issues</skos:definition>
		<fibo-fnd-utl-av:usageNote>The set of corporate actions and income events included herein are a subset of those specified in a combination of ISO 15022 Securities - Scheme for Messages (Data Field Dictionary) and the GLEIF LEI-related corporate actions. Other schemes that are specific to a custodian, depository, or regulatory agency may also be important, and should take a similar approach with respect to classification.</fibo-fnd-utl-av:usageNote>
	</owl:Class>
	
	<owl:Class rdf:about="&fibo-cae-ce-act;ActionClassifier">
		<rdfs:subClassOf rdf:resource="&fibo-fnd-arr-cls;Classifier"/>
		<rdfs:subClassOf rdf:resource="&fibo-fnd-dt-oc;OccurrenceKind"/>
		<rdfs:subClassOf>
			<owl:Restriction>
				<owl:onProperty rdf:resource="&fibo-fnd-rel-rel;isDefinedIn"/>
				<owl:onClass rdf:resource="&fibo-cae-ce-act;ActionClassificationScheme"/>
				<owl:qualifiedCardinality rdf:datatype="&xsd;nonNegativeInteger">1</owl:qualifiedCardinality>
			</owl:Restriction>
		</rdfs:subClassOf>
		<rdfs:subClassOf>
			<owl:Restriction>
				<owl:onProperty rdf:resource="&lcc-lr;isMemberOf"/>
				<owl:onClass rdf:resource="&fibo-cae-ce-act;ActionClassificationScheme"/>
				<owl:qualifiedCardinality rdf:datatype="&xsd;nonNegativeInteger">1</owl:qualifiedCardinality>
			</owl:Restriction>
		</rdfs:subClassOf>
		<rdfs:subClassOf>
			<owl:Restriction>
				<owl:onProperty rdf:resource="&lcc-cr;classifies"/>
				<owl:someValuesFrom rdf:resource="&fibo-cae-ce-act;Action"/>
			</owl:Restriction>
		</rdfs:subClassOf>
		<rdfs:subClassOf>
			<owl:Restriction>
				<owl:onProperty rdf:resource="&lcc-lr;hasTag"/>
				<owl:someValuesFrom rdf:resource="&xsd;string"/>
			</owl:Restriction>
		</rdfs:subClassOf>
		<rdfs:label xml:lang="en">action classifier</rdfs:label>
		<skos:definition xml:lang="en">classifier that distinguishes the kinds of actions and events that may be announced, initiated or carried out by an organization that affects a legal entity or the securities it issues, such as income-oriented events</skos:definition>
		<fibo-fnd-utl-av:explanatoryNote xml:lang="en">ISO 15022 classifies events as impacting income vs. others. Other classification schemes distinguish between actions that return profits to shareholders, actions that are designed to influence the share price, and actions involving a change in structure to the issuer organization.</fibo-fnd-utl-av:explanatoryNote>
	</owl:Class>
	
	<owl:Class rdf:about="&fibo-cae-ce-act;ActionStatus">
		<rdfs:subClassOf rdf:resource="&fibo-fnd-arr-lif;LifecycleStatus"/>
		<rdfs:subClassOf>
			<owl:Restriction>
				<owl:onProperty rdf:resource="&lcc-cr;classifies"/>
				<owl:someValuesFrom rdf:resource="&fibo-cae-ce-act;Action"/>
			</owl:Restriction>
		</rdfs:subClassOf>
		<rdfs:subClassOf>
			<owl:Restriction>
				<owl:onProperty rdf:resource="&lcc-lr;hasTag"/>
				<owl:someValuesFrom rdf:resource="&xsd;string"/>
			</owl:Restriction>
		</rdfs:subClassOf>
		<rdfs:label xml:lang="en">action status</rdfs:label>
		<skos:definition xml:lang="en">state of some action at some point in time</skos:definition>
	</owl:Class>
	
	<owl:Class rdf:about="&fibo-cae-ce-act;BusinessStrategyClassifier">
		<rdfs:subClassOf rdf:resource="&fibo-cae-ce-act;ActionClassifier"/>
		<rdfs:label xml:lang="en">business strategy classifier</rdfs:label>
		<skos:definition xml:lang="en">classifier of corporate actions that involve improving liquidity or changing the overall structure of the organization through diversification, combining and closing parts of the business, etc, to increase long-term profitability</skos:definition>
	</owl:Class>
	
	<owl:Class rdf:about="&fibo-cae-ce-act;ChangeAction">
		<rdfs:subClassOf rdf:resource="&fibo-cae-ce-act;MandatoryCorporateAction"/>
		<rdfs:label xml:lang="en">change action</rdfs:label>
		<skos:definition xml:lang="en">corporate action to disseminate information regarding a change further described in the corporate action details</skos:definition>
		<fibo-fnd-utl-av:explanatoryNote xml:lang="en">Generic changes may include a change in the terms of an issue, change in the identification of a security, change of board lot, change from global to definitive, etc.</fibo-fnd-utl-av:explanatoryNote>
	</owl:Class>
	
	<owl:Class rdf:about="&fibo-cae-ce-act;ClassAction">
		<rdfs:subClassOf rdf:resource="&fibo-cae-ce-act;VoluntaryCorporateAction"/>
		<rdfs:label xml:lang="en">class action</rdfs:label>
		<skos:definition xml:lang="en">corporate action involving a situation where interested parties seek restitution for financial loss</skos:definition>
		<fibo-fnd-utl-av:explanatoryNote xml:lang="en">The security holder may be offered the opportunity to join a class action proceeding and would need to respond with an instruction.</fibo-fnd-utl-av:explanatoryNote>
		<fibo-fnd-utl-av:synonym xml:lang="en">proposed settlement</fibo-fnd-utl-av:synonym>
	</owl:Class>
	
	<owl:Class rdf:about="&fibo-cae-ce-act;ConsentSolicitation">
		<rdfs:subClassOf rdf:resource="&fibo-cae-ce-act;VoluntaryCorporateAction"/>
		<rdfs:label xml:lang="en">consent solicitation</rdfs:label>
		<skos:definition xml:lang="en">corporate action that is a procedure that aims to obtain consent of holder to a proposal by the issuer or a third party without convening a meeting</skos:definition>
		<skos:example xml:lang="en">For example, consent to change the terms of a bond.</skos:example>
	</owl:Class>
	
	<owl:Class rdf:about="&fibo-cae-ce-act;CorporateAction">
		<rdfs:subClassOf rdf:resource="&fibo-cae-ce-act;Action"/>
		<rdfs:label xml:lang="en">corporate action</rdfs:label>
		<skos:definition xml:lang="en">action carried out by or specifically relating to a legal entity that may affect the securities it issues and may have a material impact on its stakeholders, such as shareholders and creditors</skos:definition>
		<skos:example xml:lang="en">Examples of corporate actions include share issues, stock splits, consolidation, dividends, mergers and acquisitions, rights issues, spin-offs, and the inception of court actions.</skos:example>
		<fibo-fnd-utl-av:explanatoryNote xml:lang="en">Corporate actions are typically approved by a company&apos;s board of directors and authorized by the shareholders.</fibo-fnd-utl-av:explanatoryNote>
	</owl:Class>
	
	<owl:Class rdf:about="&fibo-cae-ce-act;DisclosureAction">
		<rdfs:subClassOf rdf:resource="&fibo-cae-ce-act;VoluntaryCorporateAction"/>
		<rdfs:label xml:lang="en">disclosure action</rdfs:label>
		<skos:definition xml:lang="en">corporate action involving a request for holders or beneficial owners to disclose their name, location and holdings of any issue to the issuer</skos:definition>
	</owl:Class>
	
	<owl:Class rdf:about="&fibo-cae-ce-act;Divestiture">
		<rdfs:subClassOf rdf:resource="&fibo-cae-ce-act;MandatoryCorporateAction"/>
		<rdfs:label xml:lang="en">divestiture</rdfs:label>
		<skos:definition xml:lang="en">corporate action involving the sales of subsidiary business interests or investments</skos:definition>
		<skos:note xml:lang="en">Divestiture is an action or process involving the sale, spinoff, or liquidation of business assets, including product lines, services, subsidiaries, business property, or even an entire business. Companies may pursue a divestment strategy to refocus on their core business, in response to the operating environment in their industry, to raise capital, or to release underperforming assets.</skos:note>
	</owl:Class>
	
	<owl:Class rdf:about="&fibo-cae-ce-act;IncomeOrientedClassifier">
		<rdfs:subClassOf rdf:resource="&fibo-cae-ce-act;ActionClassifier"/>
		<rdfs:label xml:lang="en">income-oriented classifier</rdfs:label>
		<skos:definition xml:lang="en">classifier of corporate actions that impacts income to shareholders</skos:definition>
		<fibo-fnd-utl-av:explanatoryNote xml:lang="en">Cash dividends are a classic example where a public company declares a dividend to be paid on each outstanding share. Bonus is another case where the shareholder is rewarded. In a stricter sense, the bonus issue should not impact the share price but in reality, in rare cases, it does and results in an overall increase in value.</fibo-fnd-utl-av:explanatoryNote>
	</owl:Class>
	
	<owl:Class rdf:about="&fibo-cae-ce-act;LegalFormChange">
		<rdfs:subClassOf rdf:resource="&fibo-cae-ce-act;MandatoryCorporateAction"/>
		<rdfs:label xml:lang="en">legal form change</rdfs:label>
		<skos:definition xml:lang="en">corporate action indicating a modification of the legal form of the organization</skos:definition>
		<skos:example xml:lang="en">In the United States it is common for companies established as Subchapter S Corporations (S-Corp), typically early stage companies, to modify their structure to become full-fledged Subchapter C Corporations (C-Corp) to facilitate outside fundraising, mergers, acquisitions, and public offerings.  Other common form changes include migration from sole proprietorships to more formally registered organizations (e.g., LLC, S-Corp, C-Corp, etc.)</skos:example>
	</owl:Class>
	
	<owl:Class rdf:about="&fibo-cae-ce-act;Liquidation">
		<rdfs:subClassOf rdf:resource="&fibo-cae-ce-act;Divestiture"/>
		<rdfs:label xml:lang="en">liquidation</rdfs:label>
		<skos:definition xml:lang="en">corporate action related to winding up a business, including but not limited to distribution of cash, assets, or both</skos:definition>
		<fibo-fnd-utl-av:explanatoryNote xml:lang="en">Debt may be paid in order of priority based on preferred claims to assets specified by a security, for example.</fibo-fnd-utl-av:explanatoryNote>
	</owl:Class>
	
	<owl:Class rdf:about="&fibo-cae-ce-act;MandatoryCorporateAction">
		<rdfs:subClassOf rdf:resource="&fibo-cae-ce-act;CorporateAction"/>
		<rdfs:label xml:lang="en">mandatory corporate action</rdfs:label>
		<skos:definition xml:lang="en">action initiated by the board of directors of a corporation that affects all shareholders</skos:definition>
		<skos:example xml:lang="en">Examples of mandatory corporate actions include cash dividends, stock splits, mergers, pre-refunding, return of capital, bonus issue, asset ID change, and spin-offs.</skos:example>
		<fibo-fnd-utl-av:explanatoryNote xml:lang="en">Mandatory means mandatory participation by all shareholders, however the shareholder is not required to do anything.</fibo-fnd-utl-av:explanatoryNote>
	</owl:Class>
	
	<owl:Class rdf:about="&fibo-cae-ce-act;MandatoryWithChoiceCorporateAction">
		<rdfs:subClassOf rdf:resource="&fibo-cae-ce-act;MandatoryCorporateAction"/>
		<rdfs:label xml:lang="en">mandatory with choice corporate action</rdfs:label>
		<skos:definition xml:lang="en">mandatory corporate action where shareholders are given an opportunity to choose among several options</skos:definition>
		<fibo-fnd-utl-av:explanatoryNote xml:lang="en">In case a shareholder does not submit the election, the default option will be applied.</fibo-fnd-utl-av:explanatoryNote>
	</owl:Class>
	
	<owl:Class rdf:about="&fibo-cae-ce-act;MarketAction">
		<rdfs:subClassOf rdf:resource="&fibo-cae-ce-act;Action"/>
		<rdfs:label xml:lang="en">market action</rdfs:label>
		<skos:definition xml:lang="en">action that is initiated by a market, such as a securities exchange, that affects a legal entity or the securities it issues and may have a material impact on that entity&apos;s stakeholders, such as shareholders and creditors</skos:definition>
	</owl:Class>
	
	<owl:Class rdf:about="&fibo-cae-ce-act;MergerAcquisition">
		<rdfs:subClassOf rdf:resource="&fibo-cae-ce-act;MandatoryCorporateAction"/>
		<rdfs:label xml:lang="en">merger / acquisition</rdfs:label>
		<skos:definition xml:lang="en">corporate action involving the consolidation of legal entities or assets</skos:definition>
		<fibo-fnd-utl-av:explanatoryNote xml:lang="en">Such consolidation may be accomplished via financial transactions such as mergers, acquisitions, consolidations, tender offers, purchase of assets, and management acquisitions.</fibo-fnd-utl-av:explanatoryNote>
	</owl:Class>
	
	<owl:Class rdf:about="&fibo-cae-ce-act;Notification">
		<rdfs:subClassOf rdf:resource="&fibo-cae-ce-act;MandatoryCorporateAction"/>
		<rdfs:label xml:lang="en">notification</rdfs:label>
		<skos:definition xml:lang="en">corporate action involving information provided by the issuer having no accounting/financial impact on the holder</skos:definition>
	</owl:Class>
	
	<owl:Class rdf:about="&fibo-cae-ce-act;OrganizationAddressChange">
		<rdfs:subClassOf rdf:resource="&fibo-cae-ce-act;Notification"/>
		<rdfs:label xml:lang="en">organization address change</rdfs:label>
		<skos:definition xml:lang="en">information action that provides details of address changes for a legal entity</skos:definition>
		<skos:note xml:lang="en">Address changes may impact securities master data management, including but not limited to where shares are registered and by whom.</skos:note>
	</owl:Class>
	
	<owl:Class rdf:about="&fibo-cae-ce-act;OrganizationNameChange">
		<rdfs:subClassOf rdf:resource="&fibo-cae-ce-act;Notification"/>
		<rdfs:label xml:lang="en">organization name change</rdfs:label>
		<skos:definition xml:lang="en">information action that provides details of name changes for a legal entity</skos:definition>
		<skos:note xml:lang="en">Name changes may include legal name changes as well as &apos;doing business as&apos;, and other operational names for an organization.</skos:note>
	</owl:Class>
	
	<owl:Class rdf:about="&fibo-cae-ce-act;PriorityIssue">
		<rdfs:subClassOf rdf:resource="&fibo-cae-ce-act;VoluntaryCorporateAction"/>
		<rdfs:label xml:lang="en">priority issue</rdfs:label>
		<skos:definition xml:lang="en">corporate action that is a public offer where, due to a limited amount of securities available, priority is given to existing shareholders</skos:definition>
	</owl:Class>
	
	<owl:Class rdf:about="&fibo-cae-ce-act;RegulatoryAction">
		<rdfs:subClassOf rdf:resource="&fibo-cae-ce-act;Action"/>
		<rdfs:label xml:lang="en">regulatory action</rdfs:label>
		<skos:definition xml:lang="en">action initiated by a regulatory agency that affects a legal entity or the securities it issues and may have a material impact on that entity&apos;s stakeholders, such as shareholders and creditors</skos:definition>
	</owl:Class>
	
	<owl:Class rdf:about="&fibo-cae-ce-act;SpinOff">
		<rdfs:subClassOf rdf:resource="&fibo-cae-ce-act;Divestiture"/>
		<rdfs:label xml:lang="en">spin off</rdfs:label>
		<skos:definition xml:lang="en">corporate action involving the distribution of subsidiary stock to the shareholders of the parent company without a surrender of shares</skos:definition>
		<fibo-fnd-utl-av:explanatoryNote xml:lang="en">Spin-off represents a form of divestiture usually resulting in an independent company or in an existing company. Examples include demerger, distribution, and unbundling.</fibo-fnd-utl-av:explanatoryNote>
	</owl:Class>
	
	<owl:Class rdf:about="&fibo-cae-ce-act;VoluntaryCorporateAction">
		<rdfs:subClassOf rdf:resource="&fibo-cae-ce-act;CorporateAction"/>
		<rdfs:label xml:lang="en">voluntary corporate action</rdfs:label>
		<owl:disjointWith rdf:resource="&fibo-cae-ce-act;MandatoryCorporateAction"/>
		<skos:definition xml:lang="en">event in which the shareholders elect to participate and must respond in order for the issuer to process the action</skos:definition>
		<skos:example xml:lang="en">An example of a voluntary corporate action is a tender offer, in which the issuer may request shareholders to tender their shares at a predetermined price.</skos:example>
		<fibo-fnd-utl-av:explanatoryNote xml:lang="en">Shareholders send responses to the issuer&apos;s agents, and the issuer will send the proceeds of the action to those shareholders who elect to participate.</fibo-fnd-utl-av:explanatoryNote>
	</owl:Class>

</rdf:RDF>