<?xml version="1.0" encoding="UTF-8"?>
<!DOCTYPE rdf:RDF [
	<!ENTITY dct "http://purl.org/dc/terms/">
	<!ENTITY fibo-fnd-aap-agt "https://spec.edmcouncil.org/fibo/ontology/FND/AgentsAndPeople/Agents/">
	<!ENTITY fibo-fnd-aap-ppl "https://spec.edmcouncil.org/fibo/ontology/FND/AgentsAndPeople/People/">
	<!ENTITY fibo-fnd-org-fm "https://spec.edmcouncil.org/fibo/ontology/FND/Organizations/FormalOrganizations/">
	<!ENTITY fibo-fnd-org-org "https://spec.edmcouncil.org/fibo/ontology/FND/Organizations/Organizations/">
	<!ENTITY fibo-fnd-pty-pty "https://spec.edmcouncil.org/fibo/ontology/FND/Parties/Parties/">
	<!ENTITY fibo-fnd-pty-rl "https://spec.edmcouncil.org/fibo/ontology/FND/Parties/Roles/">
	<!ENTITY fibo-fnd-rel-rel "https://spec.edmcouncil.org/fibo/ontology/FND/Relations/Relations/">
	<!ENTITY fibo-fnd-utl-av "https://spec.edmcouncil.org/fibo/ontology/FND/Utilities/AnnotationVocabulary/">
	<!ENTITY lcc-cr "https://www.omg.org/spec/LCC/Countries/CountryRepresentation/">
	<!ENTITY lcc-lr "https://www.omg.org/spec/LCC/Languages/LanguageRepresentation/">
	<!ENTITY owl "http://www.w3.org/2002/07/owl#">
	<!ENTITY rdf "http://www.w3.org/1999/02/22-rdf-syntax-ns#">
	<!ENTITY rdfs "http://www.w3.org/2000/01/rdf-schema#">
	<!ENTITY skos "http://www.w3.org/2004/02/skos/core#">
	<!ENTITY sm "http://www.omg.org/techprocess/ab/SpecificationMetadata/">
	<!ENTITY xsd "http://www.w3.org/2001/XMLSchema#">
]>
<rdf:RDF xml:base="https://spec.edmcouncil.org/fibo/ontology/FND/Organizations/FormalOrganizations/"
	xmlns:dct="http://purl.org/dc/terms/"
	xmlns:fibo-fnd-aap-agt="https://spec.edmcouncil.org/fibo/ontology/FND/AgentsAndPeople/Agents/"
	xmlns:fibo-fnd-aap-ppl="https://spec.edmcouncil.org/fibo/ontology/FND/AgentsAndPeople/People/"
	xmlns:fibo-fnd-org-fm="https://spec.edmcouncil.org/fibo/ontology/FND/Organizations/FormalOrganizations/"
	xmlns:fibo-fnd-org-org="https://spec.edmcouncil.org/fibo/ontology/FND/Organizations/Organizations/"
	xmlns:fibo-fnd-pty-pty="https://spec.edmcouncil.org/fibo/ontology/FND/Parties/Parties/"
	xmlns:fibo-fnd-pty-rl="https://spec.edmcouncil.org/fibo/ontology/FND/Parties/Roles/"
	xmlns:fibo-fnd-rel-rel="https://spec.edmcouncil.org/fibo/ontology/FND/Relations/Relations/"
	xmlns:fibo-fnd-utl-av="https://spec.edmcouncil.org/fibo/ontology/FND/Utilities/AnnotationVocabulary/"
	xmlns:lcc-cr="https://www.omg.org/spec/LCC/Countries/CountryRepresentation/"
	xmlns:lcc-lr="https://www.omg.org/spec/LCC/Languages/LanguageRepresentation/"
	xmlns:owl="http://www.w3.org/2002/07/owl#"
	xmlns:rdf="http://www.w3.org/1999/02/22-rdf-syntax-ns#"
	xmlns:rdfs="http://www.w3.org/2000/01/rdf-schema#"
	xmlns:skos="http://www.w3.org/2004/02/skos/core#"
	xmlns:sm="http://www.omg.org/techprocess/ab/SpecificationMetadata/"
	xmlns:xsd="http://www.w3.org/2001/XMLSchema#">
	
	<owl:Ontology rdf:about="https://spec.edmcouncil.org/fibo/ontology/FND/Organizations/FormalOrganizations/">
		<rdfs:label>Formal Organizations Ontology</rdfs:label>
		<dct:abstract>This ontology defines the high level concept of formal organization for use in other FIBO ontology elements. It is purposefully underspecified to facilitate mapping to other formal organization ontologies, such as the emerging W3C formal organization ontology, or others defined for specific business and financial services standards. The concepts in this ontology extend those in the Organizations ontology.</dct:abstract>
		<dct:license rdf:datatype="&xsd;anyURI">http://opensource.org/licenses/MIT</dct:license>
		<sm:contentLanguage rdf:datatype="&xsd;anyURI">https://www.w3.org/TR/owl2-quick-reference/</sm:contentLanguage>
		<sm:copyright>Copyright (c) 2013-2022 EDM Council, Inc.</sm:copyright>
		<sm:copyright>Copyright (c) 2013-2022 Object Management Group, Inc.</sm:copyright>
		<sm:dependsOn rdf:datatype="&xsd;anyURI">https://spec.edmcouncil.org/fibo/ontology/FND/AgentsAndPeople/Agents/</sm:dependsOn>
		<sm:dependsOn rdf:datatype="&xsd;anyURI">https://spec.edmcouncil.org/fibo/ontology/FND/AgentsAndPeople/People/</sm:dependsOn>
		<sm:dependsOn rdf:datatype="&xsd;anyURI">https://spec.edmcouncil.org/fibo/ontology/FND/Organizations/Organizations/</sm:dependsOn>
		<sm:dependsOn rdf:datatype="&xsd;anyURI">https://spec.edmcouncil.org/fibo/ontology/FND/Parties/Parties/</sm:dependsOn>
		<sm:dependsOn rdf:datatype="&xsd;anyURI">https://spec.edmcouncil.org/fibo/ontology/FND/Parties/Roles/</sm:dependsOn>
		<sm:dependsOn rdf:datatype="&xsd;anyURI">https://spec.edmcouncil.org/fibo/ontology/FND/Relations/Relations/</sm:dependsOn>
		<sm:dependsOn rdf:datatype="&xsd;anyURI">https://spec.edmcouncil.org/fibo/ontology/FND/Utilities/AnnotationVocabulary/</sm:dependsOn>
		<sm:dependsOn rdf:datatype="&xsd;anyURI">https://www.omg.org/spec/LCC/</sm:dependsOn>
		<sm:fileAbbreviation>fibo-fnd-org-fm</sm:fileAbbreviation>
		<sm:filename>FormalOrganizations.rdf</sm:filename>
		<owl:imports rdf:resource="https://spec.edmcouncil.org/fibo/ontology/FND/AgentsAndPeople/Agents/"/>
		<owl:imports rdf:resource="https://spec.edmcouncil.org/fibo/ontology/FND/AgentsAndPeople/People/"/>
		<owl:imports rdf:resource="https://spec.edmcouncil.org/fibo/ontology/FND/Organizations/Organizations/"/>
		<owl:imports rdf:resource="https://spec.edmcouncil.org/fibo/ontology/FND/Parties/Parties/"/>
		<owl:imports rdf:resource="https://spec.edmcouncil.org/fibo/ontology/FND/Parties/Roles/"/>
		<owl:imports rdf:resource="https://spec.edmcouncil.org/fibo/ontology/FND/Relations/Relations/"/>
		<owl:imports rdf:resource="https://spec.edmcouncil.org/fibo/ontology/FND/Utilities/AnnotationVocabulary/"/>
		<owl:imports rdf:resource="https://www.omg.org/spec/LCC/Countries/CountryRepresentation/"/>
		<owl:imports rdf:resource="https://www.omg.org/spec/LCC/Languages/LanguageRepresentation/"/>
		<owl:versionIRI rdf:resource="https://spec.edmcouncil.org/fibo/ontology/FND/20220701/Organizations/FormalOrganizations/"/>
		<skos:changeNote>The http://www.omg.org/spec/EDMC-FIBO/FND/20130801/Organizations/FormalOrganizations.rdf version of this ontology was modified per the issue resolutions identified in the FIBO FND 1.0 FTF report and in http://www.omg.org/spec/EDMC-FIBO/FND/1.0/AboutFND-1.0/. It was further revised in the FTF in advance of the Long Beach meeting, resulting in http://www.omg.org/spec/EDMC-FIBO/FND/20141101/Organizations/FormalOrganizations/.</skos:changeNote>
		<skos:changeNote>The http://www.omg.org/spec/EDMC-FIBO/FND/20141101/Organizations/FormalOrganizations.rdf version of this ontology was modified per the FIBO 2.0 RFC to integrate concepts from LCC.</skos:changeNote>
		<skos:changeNote>The http://www.omg.org/spec/FIBO/Foundations/20130601/Organizations/FormalOrganizations.owl version of the ontology was revised in advance of the September 2013 New Brunswick, NJ meeting, as follows:
	(1) to use slash style URI/IRIss (also called 303 URIs, vs. hash style) as required to support server side processing 
	(2) to use version-independent IRIs for all definitions internally as opposed to version-specific IRIs
	(3) to change the file suffix from .owl to .rdf to increase usability in RDF tools
	(4) to use 4-level abbreviations and corresponding namespace prefixes for all FIBO ontologies, reflecting a family/specification/module/ontology structure
	(5) to incorporate changes to the specification metadata to support documentation at the family, specification, module, and ontology level, similar to the abbreviations.</skos:changeNote>
		<skos:changeNote>The https://spec.edmcouncil.org/fibo/ontology/FND/20180801/Organizations/FormalOrganizations.rdf version of this ontology was revised to loosen the constraints on the range of isDomiciledIn, allow for multiple values, update definitions to be ISO 704 compliant, and eliminate duplication with concepts in LCC.</skos:changeNote>
		<skos:changeNote>The https://spec.edmcouncil.org/fibo/ontology/FND/20200201/Organizations/FormalOrganizations.rdf version of this ontology was revised to incorporate the concept of employment, required to support regulatory reporting.</skos:changeNote>
		<skos:changeNote>The https://spec.edmcouncil.org/fibo/ontology/FND/20220101/Organizations/FormalOrganizations.rdf version of this ontology was revised to address hygiene issues with respect to text formatting.</skos:changeNote>
		<fibo-fnd-utl-av:hasMaturityLevel rdf:resource="&fibo-fnd-utl-av;Release"/>
	</owl:Ontology>
	
	<owl:Class rdf:about="&fibo-fnd-org-fm;Employee">
		<rdfs:subClassOf rdf:resource="&fibo-fnd-org-org;OrganizationMember"/>
		<rdfs:subClassOf>
			<owl:Restriction>
				<owl:onProperty rdf:resource="&fibo-fnd-org-fm;isEmployedIn"/>
				<owl:someValuesFrom rdf:resource="&fibo-fnd-org-fm;Employment"/>
			</owl:Restriction>
		</rdfs:subClassOf>
		<rdfs:subClassOf>
			<owl:Restriction>
				<owl:onProperty rdf:resource="&fibo-fnd-org-fm;isEmployeeOf"/>
				<owl:someValuesFrom rdf:resource="&fibo-fnd-org-fm;Employer"/>
			</owl:Restriction>
		</rdfs:subClassOf>
		<rdfs:subClassOf>
			<owl:Restriction>
				<owl:onProperty rdf:resource="&fibo-fnd-pty-rl;isPlayedBy"/>
				<owl:someValuesFrom rdf:resource="&fibo-fnd-aap-ppl;Person"/>
			</owl:Restriction>
		</rdfs:subClassOf>
		<rdfs:label>employee</rdfs:label>
		<rdfs:seeAlso rdf:resource="https://www.bls.gov/opub/mlr/2002/01/art1full.pdf"/>
		<skos:definition>person in the service of another under any contract of hire, express or implied, oral or written, where the employer has the right to control and direct that person in the material details of how the work is to be performed</skos:definition>
	</owl:Class>
	
	<owl:Class rdf:about="&fibo-fnd-org-fm;Employer">
		<rdfs:subClassOf rdf:resource="&fibo-fnd-org-org;MemberBearingOrganization"/>
		<rdfs:subClassOf>
			<owl:Restriction>
				<owl:onProperty rdf:resource="&fibo-fnd-org-fm;hasEmployee"/>
				<owl:someValuesFrom rdf:resource="&fibo-fnd-org-fm;Employee"/>
			</owl:Restriction>
		</rdfs:subClassOf>
		<rdfs:subClassOf>
			<owl:Restriction>
				<owl:onProperty rdf:resource="&fibo-fnd-org-fm;isEmployingParty"/>
				<owl:someValuesFrom rdf:resource="&fibo-fnd-org-fm;Employment"/>
			</owl:Restriction>
		</rdfs:subClassOf>
		<rdfs:label>employer</rdfs:label>
		<skos:definition>party that provides compensation, including wages or a salary and potentially other benefits, in exchange for work performed by one or more people, and that has the right to control and direct the employee in the material details of how the work is to be performed</skos:definition>
	</owl:Class>
	
	<owl:Class rdf:about="&fibo-fnd-org-fm;Employment">
		<rdfs:subClassOf rdf:resource="&fibo-fnd-org-org;Membership"/>
		<rdfs:subClassOf>
			<owl:Restriction>
				<owl:onProperty rdf:resource="&fibo-fnd-org-fm;hasEmployedParty"/>
				<owl:someValuesFrom rdf:resource="&fibo-fnd-org-fm;Employee"/>
			</owl:Restriction>
		</rdfs:subClassOf>
		<rdfs:subClassOf>
			<owl:Restriction>
				<owl:onProperty rdf:resource="&fibo-fnd-org-fm;hasEmployingParty"/>
				<owl:someValuesFrom rdf:resource="&fibo-fnd-org-fm;Employer"/>
			</owl:Restriction>
		</rdfs:subClassOf>
		<rdfs:label xml:lang="en">employment</rdfs:label>
		<skos:definition>situation representing the state of being employed, i.e., the relationship that holds between an employer and employee for some period of time</skos:definition>
		<skos:scopeNote>This definition does not include workers in contingent arrangements, such as independent contractors, leased employees, temporary employees, on-call workers, and others that do not have a direct contractual relationship with the employer. The distinction is important for legal reasons, particularly for regulatory reporting with respect to responsible parties such as corporate officers, lending officers, others authorized or licensed to perform certain tasks, and traders, for example.</skos:scopeNote>
		<fibo-fnd-utl-av:explanatoryNote>In the broadest sense, employment is the situation in which someone is fully engaged in doing something that they want to do. From a FIBO perspective, however, employment is understood to be more specific. It is the relationship between two parties, evidenced by an implicit or explicit contract, in which work is compensated and in which one party, a legal person, typically a formal organization, acts as the employer and the other, typically a legally capable natural person, as the employee.</fibo-fnd-utl-av:explanatoryNote>
	</owl:Class>
	
	<owl:Class rdf:about="&fibo-fnd-org-fm;FormalOrganization">
		<rdfs:subClassOf rdf:resource="&fibo-fnd-org-org;Organization"/>
		<rdfs:subClassOf>
			<owl:Restriction>
				<owl:onProperty rdf:resource="&fibo-fnd-org-fm;isDomiciledIn"/>
				<owl:someValuesFrom rdf:resource="&lcc-cr;GeopoliticalEntity"/>
			</owl:Restriction>
		</rdfs:subClassOf>
		<rdfs:label>formal organization</rdfs:label>
		<owl:disjointWith rdf:resource="&fibo-fnd-org-fm;InformalOrganization"/>
		<skos:definition>organization that is recognized in some legal jurisdiction, with associated rights and responsibilities</skos:definition>
		<skos:example>Examples include a corporation, charity, government or church.</skos:example>
		<fibo-fnd-utl-av:adaptedFrom rdf:datatype="&xsd;anyURI">https://www.w3.org/TR/vocab-org/#class-formalorganization</fibo-fnd-utl-av:adaptedFrom>
	</owl:Class>
	
	<owl:Class rdf:about="&fibo-fnd-org-fm;Group">
		<rdfs:subClassOf rdf:resource="&lcc-lr;Collection"/>
		<rdfs:subClassOf>
			<owl:Restriction>
				<owl:onProperty rdf:resource="&lcc-lr;hasMember"/>
				<owl:allValuesFrom rdf:resource="&fibo-fnd-aap-agt;AutonomousAgent"/>
			</owl:Restriction>
		</rdfs:subClassOf>
		<rdfs:label>group</rdfs:label>
		<skos:definition>collection of agents (people, organizations, software agents, etc.) that are considered as a unit</skos:definition>
	</owl:Class>
	
	<owl:Class rdf:about="&fibo-fnd-org-fm;InformalOrganization">
		<rdfs:subClassOf rdf:resource="&fibo-fnd-org-org;Organization"/>
		<rdfs:label>informal organization</rdfs:label>
		<skos:definition>organization that is not formally constituted in some way</skos:definition>
	</owl:Class>
	
	<owl:ObjectProperty rdf:about="&fibo-fnd-org-fm;employs">
		<rdfs:subPropertyOf rdf:resource="&fibo-fnd-pty-pty;playsActiveRoleThatDirectlyAffects"/>
		<rdfs:label>employs</rdfs:label>
		<rdfs:range rdf:resource="&fibo-fnd-aap-ppl;Person"/>
		<skos:definition>indicates someone that is employed by the legal person</skos:definition>
	</owl:ObjectProperty>
	
	<owl:ObjectProperty rdf:about="&fibo-fnd-org-fm;hasEmployedParty">
		<rdfs:subPropertyOf rdf:resource="&fibo-fnd-org-org;hasOrganizationMember"/>
		<rdfs:label>has employed party</rdfs:label>
		<rdfs:domain rdf:resource="&fibo-fnd-org-fm;Employment"/>
		<rdfs:range rdf:resource="&fibo-fnd-org-fm;Employee"/>
		<owl:inverseOf rdf:resource="&fibo-fnd-org-fm;isEmployedIn"/>
		<skos:definition>identifies the employee in an employment situation</skos:definition>
	</owl:ObjectProperty>
	
	<owl:ObjectProperty rdf:about="&fibo-fnd-org-fm;hasEmployee">
		<rdfs:subPropertyOf rdf:resource="&fibo-fnd-pty-pty;actsOn"/>
		<rdfs:label>has employee</rdfs:label>
		<rdfs:domain rdf:resource="&fibo-fnd-org-fm;Employer"/>
		<rdfs:range rdf:resource="&fibo-fnd-org-fm;Employee"/>
		<owl:inverseOf rdf:resource="&fibo-fnd-org-fm;isEmployeeOf"/>
		<skos:definition>indicates an employee that is employed by the employer</skos:definition>
	</owl:ObjectProperty>
	
	<owl:ObjectProperty rdf:about="&fibo-fnd-org-fm;hasEmployingParty">
		<rdfs:subPropertyOf rdf:resource="&fibo-fnd-org-org;hasMembership"/>
		<rdfs:label>has employing party</rdfs:label>
		<rdfs:domain rdf:resource="&fibo-fnd-org-fm;Employment"/>
		<rdfs:range rdf:resource="&fibo-fnd-org-fm;Employer"/>
		<owl:inverseOf rdf:resource="&fibo-fnd-org-fm;isEmployingParty"/>
		<skos:definition>identifies employer in an employment situation</skos:definition>
	</owl:ObjectProperty>
	
	<owl:ObjectProperty rdf:about="&fibo-fnd-org-fm;isDomiciledIn">
		<rdfs:label>is domiciled in</rdfs:label>
		<rdfs:domain rdf:resource="&fibo-fnd-org-fm;FormalOrganization"/>
		<rdfs:range rdf:resource="&lcc-cr;GeopoliticalEntity"/>
		<skos:definition>indicates the principal place where an entity conducts business, such as where its headquarters is located</skos:definition>
		<fibo-fnd-utl-av:explanatoryNote>Corporate domicile refers to a place where a company&apos;s affairs are discharged. It is also typically the legal home of a corporation because the place is considered by law as the center of corporate affairs. In cases where a business has incorporated in one location for convenience, such as for taxation, legal, or regulatory purposes, but operates primarily in one or more other locations, domicile in FIBO refers to the operational location(s) rather than legal location. Many companies in the US have incorporated in the State of Delaware, for example, but do not have operational facilities in Delaware (or only have small offices there).</fibo-fnd-utl-av:explanatoryNote>
	</owl:ObjectProperty>
	
	<owl:ObjectProperty rdf:about="&fibo-fnd-org-fm;isEmployedBy">
		<rdfs:subPropertyOf rdf:resource="&fibo-fnd-pty-pty;experiencesDirectly"/>
		<rdfs:label>is employed by</rdfs:label>
		<rdfs:domain rdf:resource="&fibo-fnd-aap-ppl;Person"/>
		<skos:definition>indicates the party (legal person or formal organization) that employs someone</skos:definition>
	</owl:ObjectProperty>
	
	<owl:ObjectProperty rdf:about="&fibo-fnd-org-fm;isEmployedIn">
		<rdfs:subPropertyOf rdf:resource="&fibo-fnd-org-org;isOrganizationMember"/>
		<rdfs:label>is employed in</rdfs:label>
		<rdfs:domain rdf:resource="&fibo-fnd-org-fm;Employee"/>
		<rdfs:range rdf:resource="&fibo-fnd-org-fm;Employment"/>
		<skos:definition>indicates the context of employment in which someone is employed</skos:definition>
	</owl:ObjectProperty>
	
	<owl:ObjectProperty rdf:about="&fibo-fnd-org-fm;isEmployeeOf">
		<rdfs:subPropertyOf rdf:resource="&fibo-fnd-pty-pty;isAffectedBy"/>
		<rdfs:label>is employee of</rdfs:label>
		<rdfs:domain rdf:resource="&fibo-fnd-org-fm;Employee"/>
		<rdfs:range rdf:resource="&fibo-fnd-org-fm;Employer"/>
		<skos:definition>identifies the formal organization for which the employee works</skos:definition>
	</owl:ObjectProperty>
	
	<owl:ObjectProperty rdf:about="&fibo-fnd-org-fm;isEmployingParty">
		<rdfs:subPropertyOf rdf:resource="&fibo-fnd-org-org;isMembershipPartyIn"/>
		<rdfs:label>is employing party</rdfs:label>
		<rdfs:domain rdf:resource="&fibo-fnd-org-fm;Employer"/>
		<rdfs:range rdf:resource="&fibo-fnd-org-fm;Employment"/>
		<skos:definition>relates a party in the role of employer to the context of employment</skos:definition>
	</owl:ObjectProperty>

</rdf:RDF>