<?xml version="1.0" encoding="UTF-8"?>
<!DOCTYPE rdf:RDF [
	<!ENTITY dct "http://purl.org/dc/terms/">
	<!ENTITY fibo-der-drc-bsc "https://spec.edmcouncil.org/fibo/ontology/DER/DerivativesContracts/DerivativesBasics/">
	<!ENTITY fibo-der-drc-comm "https://spec.edmcouncil.org/fibo/ontology/DER/DerivativesContracts/CommoditiesContracts/">
	<!ENTITY fibo-der-drc-ff "https://spec.edmcouncil.org/fibo/ontology/DER/DerivativesContracts/FuturesAndForwards/">
	<!ENTITY fibo-der-drc-opt "https://spec.edmcouncil.org/fibo/ontology/DER/DerivativesContracts/Options/">
	<!ENTITY fibo-der-drc-swp "https://spec.edmcouncil.org/fibo/ontology/DER/DerivativesContracts/Swaps/">
	<!ENTITY fibo-fbc-fi-fi "https://spec.edmcouncil.org/fibo/ontology/FBC/FinancialInstruments/FinancialInstruments/">
	<!ENTITY fibo-fbc-pas-fpas "https://spec.edmcouncil.org/fibo/ontology/FBC/ProductsAndServices/FinancialProductsAndServices/">
	<!ENTITY fibo-fnd-acc-cur "https://spec.edmcouncil.org/fibo/ontology/FND/Accounting/CurrencyAmount/">
	<!ENTITY fibo-fnd-agr-ctr "https://spec.edmcouncil.org/fibo/ontology/FND/Agreements/Contracts/">
	<!ENTITY fibo-fnd-arr-arr "https://spec.edmcouncil.org/fibo/ontology/FND/Arrangements/Arrangements/">
	<!ENTITY fibo-fnd-arr-cls "https://spec.edmcouncil.org/fibo/ontology/FND/Arrangements/ClassificationSchemes/">
	<!ENTITY fibo-fnd-pas-pas "https://spec.edmcouncil.org/fibo/ontology/FND/ProductsAndServices/ProductsAndServices/">
	<!ENTITY fibo-fnd-rel-rel "https://spec.edmcouncil.org/fibo/ontology/FND/Relations/Relations/">
	<!ENTITY fibo-fnd-utl-av "https://spec.edmcouncil.org/fibo/ontology/FND/Utilities/AnnotationVocabulary/">
	<!ENTITY owl "http://www.w3.org/2002/07/owl#">
	<!ENTITY rdf "http://www.w3.org/1999/02/22-rdf-syntax-ns#">
	<!ENTITY rdfs "http://www.w3.org/2000/01/rdf-schema#">
	<!ENTITY skos "http://www.w3.org/2004/02/skos/core#">
	<!ENTITY sm "http://www.omg.org/techprocess/ab/SpecificationMetadata/">
	<!ENTITY xsd "http://www.w3.org/2001/XMLSchema#">
]>
<rdf:RDF xml:base="https://spec.edmcouncil.org/fibo/ontology/DER/DerivativesContracts/CommoditiesContracts/"
	xmlns:dct="http://purl.org/dc/terms/"
	xmlns:fibo-der-drc-bsc="https://spec.edmcouncil.org/fibo/ontology/DER/DerivativesContracts/DerivativesBasics/"
	xmlns:fibo-der-drc-comm="https://spec.edmcouncil.org/fibo/ontology/DER/DerivativesContracts/CommoditiesContracts/"
	xmlns:fibo-der-drc-ff="https://spec.edmcouncil.org/fibo/ontology/DER/DerivativesContracts/FuturesAndForwards/"
	xmlns:fibo-der-drc-opt="https://spec.edmcouncil.org/fibo/ontology/DER/DerivativesContracts/Options/"
	xmlns:fibo-der-drc-swp="https://spec.edmcouncil.org/fibo/ontology/DER/DerivativesContracts/Swaps/"
	xmlns:fibo-fbc-fi-fi="https://spec.edmcouncil.org/fibo/ontology/FBC/FinancialInstruments/FinancialInstruments/"
	xmlns:fibo-fbc-pas-fpas="https://spec.edmcouncil.org/fibo/ontology/FBC/ProductsAndServices/FinancialProductsAndServices/"
	xmlns:fibo-fnd-acc-cur="https://spec.edmcouncil.org/fibo/ontology/FND/Accounting/CurrencyAmount/"
	xmlns:fibo-fnd-agr-ctr="https://spec.edmcouncil.org/fibo/ontology/FND/Agreements/Contracts/"
	xmlns:fibo-fnd-arr-arr="https://spec.edmcouncil.org/fibo/ontology/FND/Arrangements/Arrangements/"
	xmlns:fibo-fnd-arr-cls="https://spec.edmcouncil.org/fibo/ontology/FND/Arrangements/ClassificationSchemes/"
	xmlns:fibo-fnd-pas-pas="https://spec.edmcouncil.org/fibo/ontology/FND/ProductsAndServices/ProductsAndServices/"
	xmlns:fibo-fnd-rel-rel="https://spec.edmcouncil.org/fibo/ontology/FND/Relations/Relations/"
	xmlns:fibo-fnd-utl-av="https://spec.edmcouncil.org/fibo/ontology/FND/Utilities/AnnotationVocabulary/"
	xmlns:owl="http://www.w3.org/2002/07/owl#"
	xmlns:rdf="http://www.w3.org/1999/02/22-rdf-syntax-ns#"
	xmlns:rdfs="http://www.w3.org/2000/01/rdf-schema#"
	xmlns:skos="http://www.w3.org/2004/02/skos/core#"
	xmlns:sm="http://www.omg.org/techprocess/ab/SpecificationMetadata/"
	xmlns:xsd="http://www.w3.org/2001/XMLSchema#">
	
	<owl:Ontology rdf:about="https://spec.edmcouncil.org/fibo/ontology/DER/DerivativesContracts/CommoditiesContracts/">
		<rdfs:label xml:lang="en">Commodities Contracts Ontology</rdfs:label>
		<dct:abstract>This ontology specifies core concepts for commodities-based derivatives and spot contracts, including the definitions of the most common categories of underlying negotiable commodities, corresponding to those outlined in the ISO 10962 CFI standard. Note that the ontology does not include any specific units of measure for these commodities. The intent is that FIBO users would select one of the many available units ontologies to use in specifying the details of individual contracts.</dct:abstract>
		<dct:license rdf:datatype="&xsd;anyURI">http://opensource.org/licenses/MIT</dct:license>
		<sm:contentLanguage rdf:datatype="&xsd;anyURI">https://www.w3.org/TR/owl2-quick-reference/</sm:contentLanguage>
		<sm:copyright>Copyright (c) 2015-2022 EDM Council, Inc.</sm:copyright>
		<sm:copyright>Copyright (c) 2015-2022 Object Management Group, Inc.</sm:copyright>
		<sm:dependsOn rdf:resource="https://spec.edmcouncil.org/fibo/ontology/DER/DerivativesContracts/DerivativesBasics/"/>
		<sm:dependsOn rdf:resource="https://spec.edmcouncil.org/fibo/ontology/DER/DerivativesContracts/FuturesAndForwards/"/>
		<sm:dependsOn rdf:resource="https://spec.edmcouncil.org/fibo/ontology/DER/DerivativesContracts/Options/"/>
		<sm:dependsOn rdf:resource="https://spec.edmcouncil.org/fibo/ontology/DER/DerivativesContracts/Swaps/"/>
		<sm:dependsOn rdf:resource="https://spec.edmcouncil.org/fibo/ontology/FBC/"/>
		<sm:dependsOn rdf:resource="https://spec.edmcouncil.org/fibo/ontology/FND/"/>
		<sm:fileAbbreviation>fibo-der-drc-comm</sm:fileAbbreviation>
		<sm:filename>CommoditiesContracts.rdf</sm:filename>
		<owl:imports rdf:resource="https://spec.edmcouncil.org/fibo/ontology/DER/DerivativesContracts/DerivativesBasics/"/>
		<owl:imports rdf:resource="https://spec.edmcouncil.org/fibo/ontology/DER/DerivativesContracts/FuturesAndForwards/"/>
		<owl:imports rdf:resource="https://spec.edmcouncil.org/fibo/ontology/DER/DerivativesContracts/Options/"/>
		<owl:imports rdf:resource="https://spec.edmcouncil.org/fibo/ontology/DER/DerivativesContracts/Swaps/"/>
		<owl:imports rdf:resource="https://spec.edmcouncil.org/fibo/ontology/FBC/FinancialInstruments/FinancialInstruments/"/>
		<owl:imports rdf:resource="https://spec.edmcouncil.org/fibo/ontology/FBC/ProductsAndServices/FinancialProductsAndServices/"/>
		<owl:imports rdf:resource="https://spec.edmcouncil.org/fibo/ontology/FND/Accounting/CurrencyAmount/"/>
		<owl:imports rdf:resource="https://spec.edmcouncil.org/fibo/ontology/FND/Agreements/Contracts/"/>
		<owl:imports rdf:resource="https://spec.edmcouncil.org/fibo/ontology/FND/Arrangements/Arrangements/"/>
		<owl:imports rdf:resource="https://spec.edmcouncil.org/fibo/ontology/FND/Arrangements/ClassificationSchemes/"/>
		<owl:imports rdf:resource="https://spec.edmcouncil.org/fibo/ontology/FND/ProductsAndServices/ProductsAndServices/"/>
		<owl:imports rdf:resource="https://spec.edmcouncil.org/fibo/ontology/FND/Relations/Relations/"/>
		<owl:imports rdf:resource="https://spec.edmcouncil.org/fibo/ontology/FND/Utilities/AnnotationVocabulary/"/>
		<owl:versionIRI rdf:resource="https://spec.edmcouncil.org/fibo/ontology/DER/20220201/DerivativesContracts/CommoditiesContracts/"/>
		<skos:changeNote>The https://spec.edmcouncil.org/fibo/ontology/DER/20210901/DerivativesContracts/CommoditiesContracts.rdf version of this ontology was modified to fix spelling errors.</skos:changeNote>
		<skos:changeNote>The https://spec.edmcouncil.org/fibo/ontology/DER/20211201/DerivativesContracts/CommoditiesContracts.rdf version of this ontology was modified to reflect the move of precious metal from products and services to currency amount.</skos:changeNote>
		<fibo-fnd-utl-av:hasMaturityLevel rdf:resource="&fibo-fnd-utl-av;Release"/>
	</owl:Ontology>
	
	<owl:Class rdf:about="&fibo-der-drc-comm;AgriculturalResource">
		<rdfs:subClassOf rdf:resource="&fibo-fnd-pas-pas;NegotiableCommodity"/>
		<rdfs:label xml:lang="en">agricultural resource</rdfs:label>
		<skos:definition xml:lang="en">negotiable commodity that is obtained via some agricultural process, including forestry, fishing, livestock, grain, dairy, corn, cocoa, soybeans, sugar, coffee</skos:definition>
		<fibo-fnd-utl-av:adaptedFrom xml:lang="en">ISO 10962, Securities and related financial instruments - Classification of financial instruments (CFI) code, Fourth Edition, October 2019</fibo-fnd-utl-av:adaptedFrom>
	</owl:Class>
	
	<owl:Class rdf:about="&fibo-der-drc-comm;BaseMetal">
		<rdfs:subClassOf rdf:resource="&fibo-der-drc-comm;Metal"/>
		<rdfs:label xml:lang="en">base metal</rdfs:label>
		<owl:disjointWith rdf:resource="&fibo-fnd-acc-cur;PreciousMetal"/>
		<skos:definition xml:lang="en">common metal that tarnishes, oxidizes, or corrodes relatively quickly when exposed to air or moisture, that is widely used in commercial and industrial applications, such as construction and manufacturing</skos:definition>
		<fibo-fnd-utl-av:explanatoryNote xml:lang="en">Base metals or alloys include metals other than precious metals, such as copper, lead, zinc, tin, iron, steel, or brass. Note that iron and steel are included under metal and metal products in some classification schemes - see https://fred.stlouisfed.org/series/WPU101 for example.</fibo-fnd-utl-av:explanatoryNote>
	</owl:Class>
	
	<owl:Class rdf:about="&fibo-der-drc-comm;BasketOfCommodities">
		<rdfs:subClassOf rdf:resource="&fibo-fbc-pas-fpas;WeightedBasket"/>
		<rdfs:subClassOf>
			<owl:Restriction>
				<owl:onProperty rdf:resource="&fibo-fnd-arr-arr;hasConstituent"/>
				<owl:someValuesFrom rdf:resource="&fibo-der-drc-comm;CommodityBasketConstituent"/>
			</owl:Restriction>
		</rdfs:subClassOf>
		<rdfs:label>basket of commodities</rdfs:label>
		<skos:definition>custom basket whose constituents consist of one or more negotiable commodities</skos:definition>
		<fibo-fnd-utl-av:adaptedFrom xml:lang="en">ISO 10962, Securities and related financial instruments - Classification of financial instruments (CFI) code, Fourth Edition, October 2019</fibo-fnd-utl-av:adaptedFrom>
		<fibo-fnd-utl-av:explanatoryNote xml:lang="en">A commodity basket may contain constituents from one of the potential underlying assets or from multiple underlying assets.</fibo-fnd-utl-av:explanatoryNote>
	</owl:Class>
	
	<owl:Class rdf:about="&fibo-der-drc-comm;Bullion">
		<rdfs:subClassOf rdf:resource="&fibo-fnd-acc-cur;PreciousMetal"/>
		<rdfs:label xml:lang="en">bullion</rdfs:label>
		<skos:definition xml:lang="en">physical precious metal that is officially recognized as being at least 99.5 percent pure</skos:definition>
		<skos:example xml:lang="en">In the United States, bullion that is eligible for reference in a commodities contract may include U.S. gold Buffalo coins minted by the U.S. Mint that are 1 troy ounce, 0.5 ounce, 0.25 ounce, or 0.10 ounce; 1 ounce silver coins; certain platinum coins; and gold, silver, palladium, and platinum bullion that meet or exceed the fineness requirements of a regulated futures contract. Bullion must also be certified by an approved certifier, typically identified by an exchange, including but not limited to the U.S. Mint.</skos:example>
		<fibo-fnd-utl-av:explanatoryNote xml:lang="en">Physical metals fall into two categories: (1) bullion, which are coins, ingots or bars of a specific weight and purity; and (2) &quot;numismatic&quot; or collectible coins, which can be rare or old coins, or special proofs that are newly minted as collectibles. If a particular asset is identified as &quot;numismatic&quot; or &quot;collectible&quot;, it is, by definition, not considered bullion aside from its melt value.</fibo-fnd-utl-av:explanatoryNote>
	</owl:Class>
	
	<owl:Class rdf:about="&fibo-der-drc-comm;CommodityBasketConstituent">
		<rdfs:subClassOf rdf:resource="&fibo-fbc-pas-fpas;WeightedBasketConstituent"/>
		<rdfs:subClassOf>
			<owl:Restriction>
				<owl:onProperty rdf:resource="&fibo-fnd-rel-rel;comprises"/>
				<owl:someValuesFrom rdf:resource="&fibo-fnd-pas-pas;NegotiableCommodity"/>
			</owl:Restriction>
		</rdfs:subClassOf>
		<rdfs:label>commodity basket constituent</rdfs:label>
		<skos:definition>component of a custom commodity basket whose relative importance with respect to other basket constituents is known</skos:definition>
	</owl:Class>
	
	<owl:Class rdf:about="&fibo-der-drc-comm;CommodityDerivative">
		<rdfs:subClassOf rdf:resource="&fibo-fbc-fi-fi;CommodityInstrument"/>
		<rdfs:subClassOf rdf:resource="&fibo-fbc-fi-fi;DerivativeInstrument"/>
		<rdfs:subClassOf>
			<owl:Restriction>
				<owl:onProperty rdf:resource="&fibo-der-drc-bsc;hasUnderlier"/>
				<owl:onClass rdf:resource="&fibo-der-drc-comm;CommodityUnderlyingAsset"/>
				<owl:minQualifiedCardinality rdf:datatype="&xsd;nonNegativeInteger">0</owl:minQualifiedCardinality>
			</owl:Restriction>
		</rdfs:subClassOf>
		<rdfs:label>commodity derivative</rdfs:label>
		<skos:definition xml:lang="en">derivative instrument whose primary underlying notional item is a physical commodity, or the price, or related index, or any other aspect related to a physical commodity</skos:definition>
	</owl:Class>
	
	<owl:Class rdf:about="&fibo-der-drc-comm;CommodityForward">
		<rdfs:subClassOf rdf:resource="&fibo-der-drc-comm;CommodityDerivative"/>
		<rdfs:subClassOf rdf:resource="&fibo-der-drc-ff;Forward"/>
		<rdfs:label xml:lang="en">commodity forward</rdfs:label>
		<skos:definition xml:lang="en">forward contract in which a buyer and seller agree upon delivery of a specified quality and quantity of goods at a specified future date</skos:definition>
		<fibo-fnd-utl-av:adaptedFrom xml:lang="en">CFTC glossary</fibo-fnd-utl-av:adaptedFrom>
		<fibo-fnd-utl-av:adaptedFrom xml:lang="en">ISO 10962, Securities and related financial instruments - Classification of financial instruments (CFI) code, Fourth Edition, October 2019</fibo-fnd-utl-av:adaptedFrom>
		<fibo-fnd-utl-av:explanatoryNote xml:lang="en">Commodity forwards are often settled via cash transactions in many industries, including for the purposes of commodity merchandising. Terms may be more &quot;personalized&quot; than is the case with standardized futures contracts (i.e., delivery time and amount are as determined between seller and buyer). A price may be agreed upon in advance, or there may be agreement that the price will be determined at the time of delivery. A forward contract is a private and customizable agreement that settles at the end of the agreement and is traded over-the-counter.</fibo-fnd-utl-av:explanatoryNote>
	</owl:Class>
	
	<owl:Class rdf:about="&fibo-der-drc-comm;CommodityFuture">
		<rdfs:subClassOf rdf:resource="&fibo-der-drc-comm;CommodityDerivative"/>
		<rdfs:subClassOf rdf:resource="&fibo-fbc-fi-fi;Future"/>
		<rdfs:label xml:lang="en">commodity future</rdfs:label>
		<owl:disjointWith rdf:resource="&fibo-der-drc-ff;FinancialFuture"/>
		<skos:definition xml:lang="en">futures contract to buy or sell a predetermined amount of a commodity at a specific price on a specific date in the future</skos:definition>
		<fibo-fnd-utl-av:adaptedFrom xml:lang="en">CFTC glossary</fibo-fnd-utl-av:adaptedFrom>
		<fibo-fnd-utl-av:adaptedFrom xml:lang="en">ISO 10962, Securities and related financial instruments - Classification of financial instruments (CFI) code, Fourth Edition, October 2019</fibo-fnd-utl-av:adaptedFrom>
		<fibo-fnd-utl-av:explanatoryNote xml:lang="en">A commodity future is an agreement to purchase or sell a commodity for delivery in the future: (1) at a price that is determined at initiation of the contract; (2) that obligates each party to the contract to fulfill the contract at the specified price; (3) that is used to assume or shift price risk; and (4) that may be satisfied by delivery or offset.</fibo-fnd-utl-av:explanatoryNote>
	</owl:Class>
	
	<owl:Class rdf:about="&fibo-der-drc-comm;CommodityOption">
		<rdfs:subClassOf rdf:resource="&fibo-der-drc-comm;CommodityDerivative"/>
		<rdfs:subClassOf rdf:resource="&fibo-der-drc-opt;VanillaOption"/>
		<rdfs:label xml:lang="en">commodity option</rdfs:label>
		<skos:definition xml:lang="en">option where the option buyer has the right to buy or sell specified commodities or commodity related index at a fixed price or formula, on or before a specified date</skos:definition>
		<fibo-fnd-utl-av:adaptedFrom xml:lang="en">ISO 10962, Securities and related financial instruments - Classification of financial instruments (CFI) code, Fourth Edition, October 2019</fibo-fnd-utl-av:adaptedFrom>
	</owl:Class>
	
	<owl:Class rdf:about="&fibo-der-drc-comm;CommodityReturnLeg">
		<rdfs:subClassOf rdf:resource="&fibo-der-drc-swp;ReturnLeg"/>
		<rdfs:subClassOf>
			<owl:Restriction>
				<owl:onProperty rdf:resource="&fibo-der-drc-bsc;hasUnderlier"/>
				<owl:someValuesFrom rdf:resource="&fibo-der-drc-comm;CommodityUnderlyingAsset"/>
			</owl:Restriction>
		</rdfs:subClassOf>
		<rdfs:label xml:lang="en">commodity return leg</rdfs:label>
		<skos:definition xml:lang="en">leg of a commodity return swap in which the return is based on a physical commodity, or the price, or behavior of the price, or any other aspect related to a physical commodity</skos:definition>
		<fibo-fnd-utl-av:explanatoryNote xml:lang="en">The cash flows from a commodity may be negative as you have a cost from holding the commodity but there are no interim cash flows, so it equates to a negative interest rate. So a commodity swap is like a TRS in that it is based on the return on the increase in value.</fibo-fnd-utl-av:explanatoryNote>
	</owl:Class>
	
	<owl:Class rdf:about="&fibo-der-drc-comm;CommoditySpotContract">
		<rdfs:subClassOf rdf:resource="&fibo-fbc-fi-fi;CommodityInstrument"/>
		<rdfs:subClassOf rdf:resource="&fibo-fbc-fi-fi;SpotContract"/>
		<rdfs:subClassOf>
			<owl:Restriction>
				<owl:onProperty rdf:resource="&fibo-fnd-rel-rel;involves"/>
				<owl:someValuesFrom rdf:resource="&fibo-fnd-pas-pas;NegotiableCommodity"/>
			</owl:Restriction>
		</rdfs:subClassOf>
		<rdfs:label xml:lang="en">commodity spot contract</rdfs:label>
		<skos:definition xml:lang="en">The contract defined for or implied in a Commodities spot transaction.</skos:definition>
	</owl:Class>
	
	<owl:Class rdf:about="&fibo-der-drc-comm;CommoditySwap">
		<rdfs:subClassOf rdf:resource="&fibo-der-drc-comm;CommodityDerivative"/>
		<rdfs:subClassOf rdf:resource="&fibo-der-drc-swp;ReturnSwap"/>
		<rdfs:subClassOf>
			<owl:Restriction>
				<owl:onProperty rdf:resource="&fibo-der-drc-swp;hasReturnLeg"/>
				<owl:someValuesFrom rdf:resource="&fibo-der-drc-comm;CommodityReturnLeg"/>
			</owl:Restriction>
		</rdfs:subClassOf>
		<rdfs:label xml:lang="en">commodity swap</rdfs:label>
		<skos:definition xml:lang="en">commodity derivative that includes, without limitation, any swap for which the primary underlying notional item is a physical commodity, or the price, or behavior of the price, or the level of a commodity index, or other aspect related to a physical commodity</skos:definition>
		<fibo-fnd-utl-av:adaptedFrom xml:lang="en">CFTC glossary</fibo-fnd-utl-av:adaptedFrom>
		<fibo-fnd-utl-av:adaptedFrom xml:lang="en">ISO 10962, Securities and related financial instruments - Classification of financial instruments (CFI) code, Fourth Edition, October 2019</fibo-fnd-utl-av:adaptedFrom>
		<fibo-fnd-utl-av:explanatoryNote xml:lang="en">Commodity swaps typically involve the exchange of a floating commodity price for a set price over an agreed-upon period.</fibo-fnd-utl-av:explanatoryNote>
	</owl:Class>
	
	<owl:Class rdf:about="&fibo-der-drc-comm;CommodityUnderlyingAsset">
		<rdfs:subClassOf rdf:resource="&fibo-der-drc-bsc;Underlier"/>
		<rdfs:subClassOf>
			<owl:Restriction>
				<owl:onProperty rdf:resource="&fibo-fnd-rel-rel;hasIdentity"/>
				<owl:someValuesFrom rdf:resource="&fibo-fnd-pas-pas;NegotiableCommodity"/>
			</owl:Restriction>
		</rdfs:subClassOf>
		<rdfs:label>commodity underlying asset</rdfs:label>
		<skos:definition xml:lang="en">underlier of a commodity derivative, including, but not limited to, the negotiable commodity itself</skos:definition>
		<fibo-fnd-utl-av:explanatoryNote xml:lang="en">The underlying of a commodity swap may include a physical commodity, or the price, or behavior of the price, or any other aspect of a physical commodity.</fibo-fnd-utl-av:explanatoryNote>
	</owl:Class>
	
	<owl:Class rdf:about="&fibo-der-drc-comm;EnergyResource">
		<rdfs:subClassOf rdf:resource="&fibo-fnd-pas-pas;NegotiableCommodity"/>
		<rdfs:label xml:lang="en">energy resource</rdfs:label>
		<skos:definition xml:lang="en">negotiable commodity that is an energy-related product, or a derivative of an energy-related product, including electricity, renewable energy, or any power/energy delivered through a utility network of provider; diesel fuel, fuel oil, gas oil, gasoline, heating oil, jet fuel, kerosene, natural gas, oil (Brent, Tapis, Dubai, WTI)</skos:definition>
		<skos:scopeNote xml:lang="en">Note that the concept of an energy resource overlaps with generated resource and extraction resource but is not identical to either.</skos:scopeNote>
		<fibo-fnd-utl-av:adaptedFrom xml:lang="en">ISO 10962, Securities and related financial instruments - Classification of financial instruments (CFI) code, Fourth Edition, October 2019</fibo-fnd-utl-av:adaptedFrom>
	</owl:Class>
	
	<owl:Class rdf:about="&fibo-der-drc-comm;EnergyTransmissionRights">
		<rdfs:subClassOf rdf:resource="&fibo-der-drc-comm;EnergyResource"/>
		<rdfs:label xml:lang="en">energy transmission rights</rdfs:label>
		<skos:definition xml:lang="en">rights to the transmission of power across an electricity distribution network</skos:definition>
	</owl:Class>
	
	<owl:Class rdf:about="&fibo-der-drc-comm;EnvironmentalResource">
		<rdfs:subClassOf rdf:resource="&fibo-fnd-pas-pas;NegotiableCommodity"/>
		<rdfs:label xml:lang="en">environmental resource</rdfs:label>
		<skos:definition xml:lang="en">negotiable commodity including offset credits</skos:definition>
		<fibo-fnd-utl-av:adaptedFrom xml:lang="en">ISO 10962, Securities and related financial instruments - Classification of financial instruments (CFI) code, Fourth Edition, October 2019</fibo-fnd-utl-av:adaptedFrom>
	</owl:Class>
	
	<owl:Class rdf:about="&fibo-der-drc-comm;ExtractionResource">
		<rdfs:subClassOf rdf:resource="&fibo-fnd-pas-pas;NegotiableCommodity"/>
		<rdfs:label xml:lang="en">extraction resource</rdfs:label>
		<skos:definition xml:lang="en">negotiable commodity that is a mineral resource obtained via withdrawal from the natural environment</skos:definition>
		<fibo-fnd-utl-av:adaptedFrom xml:lang="en">ISO 10962, Securities and related financial instruments - Classification of financial instruments (CFI) code, Fourth Edition, October 2019</fibo-fnd-utl-av:adaptedFrom>
		<fibo-fnd-utl-av:explanatoryNote xml:lang="en">These resources include ores, which contain commercially valuable amounts of metals, such as iron and aluminum, as well as precious metals, such as silver, gold, and platinum; precious stones, such as diamonds; building stones, such as granite; and solid fuels, such as coal and oil shale.</fibo-fnd-utl-av:explanatoryNote>
	</owl:Class>
	
	<owl:Class rdf:about="&fibo-der-drc-comm;FertilizerResource">
		<rdfs:subClassOf rdf:resource="&fibo-fnd-pas-pas;NegotiableCommodity"/>
		<rdfs:label xml:lang="en">fertilizer resource</rdfs:label>
		<skos:definition xml:lang="en">negotiable commodity that includes ammonia, diammonium phosphate (DAP), potash, sulphur, urea, urea and ammonium nitrate (UAN)</skos:definition>
		<fibo-fnd-utl-av:adaptedFrom xml:lang="en">ISO 10962, Securities and related financial instruments - Classification of financial instruments (CFI) code, Fourth Edition, October 2019</fibo-fnd-utl-av:adaptedFrom>
	</owl:Class>
	
	<owl:Class rdf:about="&fibo-der-drc-comm;FreightResource">
		<rdfs:subClassOf rdf:resource="&fibo-fnd-pas-pas;NegotiableCommodity"/>
		<rdfs:label xml:lang="en">freight resource</rdfs:label>
		<skos:definition xml:lang="en">negotiable commodity that is a freight index route</skos:definition>
		<fibo-fnd-utl-av:adaptedFrom xml:lang="en">ISO 10962, Securities and related financial instruments - Classification of financial instruments (CFI) code, Fourth Edition, October 2019</fibo-fnd-utl-av:adaptedFrom>
	</owl:Class>
	
	<owl:Class rdf:about="&fibo-der-drc-comm;GasCommodity">
		<rdfs:subClassOf rdf:resource="&fibo-der-drc-comm;EnergyResource"/>
		<rdfs:subClassOf rdf:resource="&fibo-der-drc-comm;ExtractionResource"/>
		<rdfs:label xml:lang="en">gas commodity</rdfs:label>
		<skos:definition xml:lang="en">extraction resource that is natural gas</skos:definition>
	</owl:Class>
	
	<owl:Class rdf:about="&fibo-der-drc-comm;GeneratedResource">
		<rdfs:subClassOf rdf:resource="&fibo-fnd-pas-pas;NegotiableCommodity"/>
		<rdfs:label xml:lang="en">generated resource</rdfs:label>
		<skos:definition xml:lang="en">negotiable commodity obtained via some generation process, including electricity, renewable energy, or any power/energy delivered through a utility network or provider</skos:definition>
		<fibo-fnd-utl-av:adaptedFrom xml:lang="en">ISO 10962, Securities and related financial instruments - Classification of financial instruments (CFI) code, Fourth Edition, October 2019</fibo-fnd-utl-av:adaptedFrom>
	</owl:Class>
	
	<owl:Class rdf:about="&fibo-der-drc-comm;GrainCommodity">
		<rdfs:subClassOf rdf:resource="&fibo-der-drc-comm;AgriculturalResource"/>
		<rdfs:label xml:lang="en">grain commodity</rdfs:label>
		<skos:definition xml:lang="en">agricultural resource that is a small, hard seed, of a food plant, especially of a cereal plant, such as wheat, corn, rye, oats, rice, and millet</skos:definition>
	</owl:Class>
	
	<owl:Class rdf:about="&fibo-der-drc-comm;IndustrialResource">
		<rdfs:subClassOf rdf:resource="&fibo-fnd-pas-pas;NegotiableCommodity"/>
		<rdfs:label xml:lang="en">industrial resource</rdfs:label>
		<skos:definition xml:lang="en">negotiable commodity that is obtained via some industrial process, including construction and manufacturing</skos:definition>
		<fibo-fnd-utl-av:adaptedFrom xml:lang="en">ISO 10962, Securities and related financial instruments - Classification of financial instruments (CFI) code, Fourth Edition, October 2019</fibo-fnd-utl-av:adaptedFrom>
	</owl:Class>
	
	<owl:Class rdf:about="&fibo-der-drc-comm;MeatCommodity">
		<rdfs:subClassOf rdf:resource="&fibo-der-drc-comm;AgriculturalResource"/>
		<rdfs:label xml:lang="en">meat commodity</rdfs:label>
		<skos:definition xml:lang="en">agricultural resource derived from the flesh of an animal (especially a mammal), such as pork bellies</skos:definition>
	</owl:Class>
	
	<owl:Class rdf:about="&fibo-der-drc-comm;Metal">
		<rdfs:subClassOf rdf:resource="&fibo-der-drc-comm;ExtractionResource"/>
		<rdfs:label xml:lang="en">metal</rdfs:label>
		<skos:definition xml:lang="en">material that, when freshly prepared, polished, or fractured, shows a lustrous appearance, and conducts electricity and heat relatively well</skos:definition>
		<skos:example xml:lang="en">Examples include precious or industrial metal, such as aluminium, copper, gold, lead, nickel, platinum, silver, tin, zinc.</skos:example>
		<fibo-fnd-utl-av:adaptedFrom xml:lang="en">ISO 10962, Securities and related financial instruments - Classification of financial instruments (CFI) code, Fourth Edition, October 2019</fibo-fnd-utl-av:adaptedFrom>
		<fibo-fnd-utl-av:adaptedFrom xml:lang="en">https://en.wikipedia.org/wiki/Metal</fibo-fnd-utl-av:adaptedFrom>
	</owl:Class>
	
	<owl:Class rdf:about="&fibo-der-drc-comm;OilCommodity">
		<rdfs:subClassOf rdf:resource="&fibo-der-drc-comm;GeneratedResource"/>
		<rdfs:subClassOf>
			<owl:Restriction>
				<owl:onProperty rdf:resource="&fibo-der-drc-comm;hasGrade"/>
				<owl:someValuesFrom rdf:resource="&fibo-der-drc-comm;OilGrade"/>
			</owl:Restriction>
		</rdfs:subClassOf>
		<rdfs:label xml:lang="en">oil commodity</rdfs:label>
		<skos:definition xml:lang="en">generated resource that is a viscous liquid derived from petroleum, including for use as fuel, or as a lubricant, and the manufacture of many types of paints, plastics, and other materials</skos:definition>
	</owl:Class>
	
	<owl:Class rdf:about="&fibo-der-drc-comm;OilGrade">
		<rdfs:subClassOf rdf:resource="&fibo-fnd-arr-cls;Classifier"/>
		<rdfs:label xml:lang="en">oil grade</rdfs:label>
		<skos:definition xml:lang="en">measure of the viscosity of oil during operation</skos:definition>
	</owl:Class>
	
	<owl:Class rdf:about="&fibo-der-drc-comm;PaperResource">
		<rdfs:subClassOf rdf:resource="&fibo-fnd-pas-pas;NegotiableCommodity"/>
		<rdfs:label xml:lang="en">paper resource</rdfs:label>
		<skos:definition xml:lang="en">negotiable commodity that is a paper product, including containerboard, newsprint, pulp, recovered paper</skos:definition>
		<fibo-fnd-utl-av:adaptedFrom xml:lang="en">ISO 10962, Securities and related financial instruments - Classification of financial instruments (CFI) code, Fourth Edition, October 2019</fibo-fnd-utl-av:adaptedFrom>
	</owl:Class>
	
	<owl:Class rdf:about="&fibo-der-drc-comm;PolypropyleneResource">
		<rdfs:subClassOf rdf:resource="&fibo-fnd-pas-pas;NegotiableCommodity"/>
		<rdfs:label xml:lang="en">polypropylene resource</rdfs:label>
		<skos:definition xml:lang="en">negotiable commodity including plastics</skos:definition>
		<fibo-fnd-utl-av:adaptedFrom xml:lang="en">ISO 10962, Securities and related financial instruments - Classification of financial instruments (CFI) code, Fourth Edition, October 2019</fibo-fnd-utl-av:adaptedFrom>
	</owl:Class>
	
	<owl:Class rdf:about="&fibo-der-drc-comm;ServiceResource">
		<rdfs:subClassOf rdf:resource="&fibo-fnd-pas-pas;NegotiableCommodity"/>
		<rdfs:label xml:lang="en">service resource</rdfs:label>
		<skos:definition xml:lang="en">negotiable commodity involving services such as transportation, communications, and trade</skos:definition>
		<fibo-fnd-utl-av:adaptedFrom xml:lang="en">ISO 10962, Securities and related financial instruments - Classification of financial instruments (CFI) code, Fourth Edition, October 2019</fibo-fnd-utl-av:adaptedFrom>
	</owl:Class>
	
	<owl:Class rdf:about="&fibo-der-drc-comm;WeatherDerivative">
		<rdfs:subClassOf rdf:resource="&fibo-der-drc-comm;CommodityDerivative"/>
		<rdfs:subClassOf rdf:resource="&fibo-fbc-fi-fi;DerivativeInstrument"/>
		<rdfs:label>weather derivative</rdfs:label>
		<skos:definition xml:lang="en">derivative instrument whose primary underlying notional item is based on something related to the weather, for example, the average temperature in Chicago in January</skos:definition>
		<fibo-fnd-utl-av:adaptedFrom xml:lang="en">CFTC glossary, https://www.cftc.gov/LearnAndProtect/EducationCenter/CFTCGlossary/glossary_wxyz.html</fibo-fnd-utl-av:adaptedFrom>
		<fibo-fnd-utl-av:explanatoryNote xml:lang="en">In the CFI standard, weather is classified as an environmental resource.</fibo-fnd-utl-av:explanatoryNote>
		<fibo-fnd-utl-av:explanatoryNote xml:lang="en">Such a derivative can be used to hedge risks related to the demand for heating fuel or electricity. The underlying &apos;asset&apos; is not a negotiable commodity per se, but because the weather can impact the prices and other things related to other commodities, weather derivatives are treated as commodity derivatives for regulatory purposes.</fibo-fnd-utl-av:explanatoryNote>
	</owl:Class>
	
	<owl:ObjectProperty rdf:about="&fibo-der-drc-comm;hasGrade">
		<rdfs:label xml:lang="en">has grade</rdfs:label>
		<rdfs:domain rdf:resource="&fibo-der-drc-comm;OilCommodity"/>
		<rdfs:range rdf:resource="&fibo-der-drc-comm;OilGrade"/>
		<skos:definition xml:lang="en">The grade of oil e.g. Brent Crude.</skos:definition>
	</owl:ObjectProperty>
	
	<owl:Class rdf:about="&fibo-fnd-acc-cur;PreciousMetal">
		<rdfs:subClassOf rdf:resource="&fibo-der-drc-comm;Metal"/>
	</owl:Class>

</rdf:RDF>